src/Init/Data/Vector.lean
@@ -5,3 +5,5 @@ Authors: Kim Morrison
 -/
 prelude
 import Init.Data.Vector.Basic
+import Init.Data.Vector.Lemmas
+import Init.Data.Vector.MapIdx
